

Honor Mathematics Lecture 2 Solution

From Numbers to Sequences – Exercises

“Practice makes Perfect...”

Pingbang Hu

University of Michigan

October 29, 2021



JOINT INSTITUTE
交大密西根学院

1. When learning the axioms of rational number, one student found that the operation of subsets of a non-empty set X is somewhat similar to that of rational number:

If we regard \cup as $+$, \cap as \cdot , then the equation

$$A \cap (B \cup C) = (A \cap B) \cup (A \cap C)$$

is just the distributivity law. Help him check whether P1 – P9 also hold for such operations.

We check by enumerating P1 – P9.

1. $A \cup (B \cup C) = (A \cup B) \cup C$
2. $A \cup \emptyset = \emptyset \cup A = A$
3. $A \cup B = B \cup A$
4. $A^c \cup A = A \cup A^c = X$
5. $A \cap (B \cap C) = (A \cap B) \cap C$
6. $A \cap X = X \cap A = A$
7. $A \cap B = B \cap A$
8. $A \cap \emptyset = \emptyset \cap A = \emptyset$
9. $A \cap (B \cup C) = (A \cap B) \cup (A \cap C)$

As we can see, P4 and P8 does not hold, since we can't find the inverse element for \cup and \cap , so the answer of this exercise is no. ■

2.

1. Prove that for $a_i \in \mathbb{Q}, i \in \mathbb{N}^*$, and n is a natural number,

$$\left| \sum_{i=1}^n a_i \right| \leq \sum_{i=1}^n |a_i|$$

2. Prove that $|a - c| \leq |a - b| + |c - b|$

2 - 1

Proof :

$$\left| \sum_{i=1}^n a_i \right| = |a_1 + a_2 + \cdots + a_n| = |(a_1 + \cdots + a_{n-1}) + a_n|$$

$$\leq |a_1 + \cdots + a_{n-1}| + |a_n| \leq \dots$$

.

.

.

$$\leq |a_1| + |a_2| + \cdots + |a_n| = \sum_{i=1}^n |a_i|$$



$2 - 2$

Proof :

$$\begin{aligned}|a - c| &= |a + b - b - c| \\&= |(a - b) + (b - c)| \\&\leq |a - b| + |b - c| \\&= |a - b| + |c - b|\end{aligned}$$



3. We define \mathbb{R} as a set containing rational numbers and the limits of rational numbers. Let $E \subseteq \mathbb{R}$ a non-empty subset of that is bounded above in \mathbb{R} . Now we don't assume P13 is an axiom. We want to prove P13 with P1 – P12 and other facts that we know:

- ▶ Let's call the set of form $(a, +\infty)$ or $[a, +\infty)$ *up interval*. Prove that the set of E 's upper bound, denoted by U , is an *up interval*.
- ▶ (**Theorem 2.2**) E has a least upper bound.

3 – 1

Proof :

We first prove that U is an interval by contradiction. Suppose U is not an interval, then we can see

$$\exists m \notin U \quad \begin{cases} U \cap (-\infty, m) \neq \emptyset \\ U \cap (m, \infty) \neq \emptyset \end{cases}$$

From here, we have two useful conditions as follows.

1. Since $m \notin U$, $\exists_{x \in E} x > m$.

2. Since $(-\infty, m) \cap U \neq \emptyset$, $\exists y \in (-\infty, m) \cap U \Rightarrow \begin{cases} y < m \\ y \in U \end{cases}$

Finally, we get $y < m < x$, but this is a contradiction since y is an upper bound but $y < x \in E$.

3 – 1

Proof(continue) :

Then, we know U is an interval now. Because U is clearly bounded below by some element in E , let say a , then U should have this form:

$$U = (a, b) \text{ or } U = [a, b)$$

for some b . And because if $b \in U$, then clearly $b + c \in U$ for $c > 0$, we know that

$$U = (a, \infty) \text{ or } U = [a, \infty)$$

so U is an up interval. ■

3 - 2

Proof :

We consider two cases.


First, if $U = [a, \infty)$, then clearly, U has a minimum a , and which is the least upper bound of E .

Second, if $U = (a, \infty)$, then we know

$$\begin{cases} \exists_{x \in E} x > a \Rightarrow \exists_{\epsilon > 0} x = a + 2\epsilon \\ \forall_{\epsilon > 0} a + \epsilon \in U \Rightarrow a + \epsilon > x \end{cases}$$

We simply fixed the ϵ we found in equation 1, and then plug in to the equation 2, we get

$$a + \epsilon > x = a + 2\epsilon \Rightarrow \epsilon < 0$$

Which contradicts to our chosen condition of ϵ , so we know the second case $U = (a, \infty)$ can not be the case. 

4. Let A be bounded set in \mathbb{R} (which means that the total set is \mathbb{R}), for any $\epsilon > 0$, there is an element x in A such that $|x - \sup A| < \epsilon$.

4

Proof :

We proceed our proof by contradiction. Suppose this is not true, namely there is an $\epsilon > 0$ such that for all $x \in A$ we have

$$|x - \sup A| \geq \epsilon$$

But then we know, $\sup A - \frac{1}{2}\epsilon$ is an upper bound of A , which leads to a contradiction. ■

5. A sequence is defined as

$$(S_n)_{n \in \mathbb{N}}, \quad S_1 = \sqrt{2}, \quad S_2 = \sqrt{2\sqrt{2}}, \quad S_3 = \sqrt{2\sqrt{2\sqrt{2}}}$$

Please calculate the limit of (S_n) as $n \rightarrow \infty$, if it exists.

5.

Since we don't know whether the limit of (S_n) exist or not, we must first prove the existence, then do the following calculation.

We proceed as follows. First, we observe that (S_n) is bounded since

$$0 \leq S_n = \underbrace{\sqrt{2\sqrt{2\sqrt{2\ldots\sqrt{2}}}}}_{n \text{ square roots}} \leq \underbrace{\sqrt{2\sqrt{2\sqrt{2\ldots 2}}}}_{n \text{ square roots}} = 2$$

We get the right-hand side by replacing the last $\sqrt{2}$ by 2 from the left-hand side.

We conclude that the sequence (S_n) is bounded. Our goal is to prove (S_n) is convergent, so we now only need to prove (S_n) is monotonic, then we can deduce the convergence from our already known lemma.

(continue)

Since $S_{n+1} = \sqrt{2S_n}$ for $n \geq 1$. When $n \geq 1$,

$$\frac{S_{n+1}}{S_n} = \frac{\sqrt{2S_n}}{S_n} = \frac{\sqrt{2}}{\sqrt{S_n}} > \frac{\sqrt{2}}{\sqrt{2}} = 1$$

It is easy to see that (S_n) is strictly increasing, which means it is monotonic, hence convergent.

To calculate the limit, we use the equation

$$\lim_{n \rightarrow \infty} S_{n+1} = \lim_{n \rightarrow \infty} S_n =: L$$

Which leads to $\sqrt{2L} = L$. By solving this equation and the fact that $S_n \geq S_1 = 1$, so $L = 2$, which mean the limit is 2. ■

6. Let $(a_n), (b_n)$ be two real sequences. Furthermore, assume that $a_n < b_n$ for all n , $[a_{n+1}, b_{n+1}] \subseteq [a_n, b_n]$, $\lim(a_n - b_n) = 0$. Prove that there is a unique $m \in [a_n, b_n]$ for all n , such that

$$\lim a_n = \lim b_n = m$$

6.

Proof :

We first show that $(a_n), (b_n)$ are convergent. Notice that $[a_{n+1}, b_{n+1}] \subseteq [a_n, b_n]$ means that (a_n) is increasing, while (b_n) is decreasing. Furthermore, both (a_n) and (b_n) are bounded by $[a_0, b_0]$. Therefore, (a_n) and (b_n) are convergent.

Next we show that $\lim a_n = \lim b_n$. Suppose $\lim b_n = L$, where L is a unique number since a sequence has precisely one limit. Then we know

$$\lim a_n = \lim[(a_n - b_n) + b_n] = \lim(a_n - b_n) + \lim b_n = 0 + L = L$$

Moreover, since $\begin{cases} L \geq a_n \\ L \leq b_n \end{cases}$, we know that $L \in [a_n, b_n]$. ■

7. Let (x_n) be a bounded real sequence. Then define

$$a_n := \sup_{m \geq n} (x_m), \quad b_n := \inf_{m \geq n} (x_m)$$

1. Prove that (a_n) is decreasing, while (b_n) is increasing.
2. Since both $(a_n), (b_n)$ are monotonic and bounded, they are convergent. We denote $\underline{\lim} x_n = \lim b_n$; $\overline{\lim} x_n = \lim a_n$. Show that:

$$\underline{\lim} y_n + \underline{\lim} z_n \leq \underline{\lim} (y_n + z_n) \leq \overline{\lim} y_n + \underline{\lim} z_n \leq \overline{\lim} y_n + \overline{\lim} z_n$$

7 – 1

Proof :

This follows from the fact that for two bounded sets A, B in \mathbb{R} with $A \supseteq B$, the supremum of A is no less than the supremum of B . Similarly, for two bounded sets A, B in \mathbb{R} with $A \supseteq B$, the infimum of A is no greater than the infimum of B .

7 - 2

Proof :

We precede from the left-hand side. Start from the first inequality:

$$\underline{\lim} y_n + \underline{\lim} z_n \leq \underline{\lim} (y_n + z_n)$$

Fix $\epsilon > 0$, there is an $M \in \mathbb{N}$ such that $\forall_{n \geq M} y_n \geq \underline{\lim} y_n - \frac{\epsilon}{4}$, and $z_n \geq \underline{\lim} z_n - \frac{\epsilon}{4}$. So we have $\underline{\lim} y_n + \underline{\lim} z_n - \frac{\epsilon}{2} \leq (y_n + z_n)$ for all such n . Next, we claim that there is always a subsequence of $(y_n + z_n)$ such that it converges to $\underline{\lim} (y_n + z_n)$.

Fix arbitrary $t > 0$, $\forall_{M \in \mathbb{N}} \exists_{n_k \geq M}$ such that

$$\begin{cases} |(y_{n_k} + z_{n_k}) - \inf_{m \geq M} (y_m + z_m)| < \frac{1}{2}t \\ |(y_{n_k} + z_{n_k}) - \underline{\lim} (y_n + z_n)| < \frac{1}{2}t \end{cases}$$

7 - 2

Proof(continue) :

We know $|(y_{n_k} + z_{n_k}) - \underline{\lim}(y_n + z_n)| < t$. This means for large enough n_k (at least $n_k > M$) we make sure that $(y_{n_k} + z_{n_k}) \leq \underline{\lim}(y_n + z_n) + \frac{\epsilon}{2}$ and also

$$\underline{\lim}y_n + \underline{\lim}z_n - \frac{\epsilon}{2} \leq (y_{n_k} + z_{n_k}) \leq \underline{\lim}(y_n + z_n) + \frac{\epsilon}{2}$$

$$\Rightarrow \underline{\lim}y_n + \underline{\lim}z_n \leq \underline{\lim}(y_n + z_n) + \epsilon$$

Since this is true for all $\epsilon > 0$, we conclude that

$$\underline{\lim}y_n + \underline{\lim}z_n \leq \underline{\lim}(y_n + z_n)$$

7 – 2

Proof(continue) :

Now we prove the second inequality.

$$\underline{\lim}(y_n + z_n) \leq \overline{\lim}y_n + \underline{\lim}z_n$$

From the fact that

$$-\underline{\lim}(-x_n) = \overline{\lim}x_n$$

This equality holds because $-\inf_{m \geq n}(-x_m) = \sup_{m \geq n} x_m$. Now, $\underline{\lim}(y_n + z_n) + \underline{\lim}(-y_n) \leq \underline{\lim}(y_n + z_n + (-y_n)) = \underline{\lim}z_n$ by what we have proved above. Thus,

$$\underline{\lim}(y_n + z_n) \leq -\underline{\lim}(-y_n) + \underline{\lim}z_n = \overline{\lim}y_n + \underline{\lim}z_n$$

7 – 2

Proof(continue) :

Finally, we now prove the last inequality.

$$\overline{\lim} y_n + \underline{\lim} z_n \leq \overline{\lim} y_n + \overline{\lim} z_n$$

Since $a_n := \sup_{m \geq n} x_m \geq \inf_{m \geq n} x_m =: b_n$, we have

$$\underline{\lim} z_n \leq \overline{\lim} z_n$$

Therefore,

$$\overline{\lim} y_n + \underline{\lim} z_n \leq \overline{\lim} y_n + \overline{\lim} z_n$$



8. Let (a_n) be a sequence such that

$$a_n = \frac{1}{\sqrt{n^2 + 1}} + \cdots + \frac{1}{\sqrt{n^2 + n}}$$

Calculate the limit of (a_n) .

8.

We first consider two sequence $(b_n)_{n \geq 1}, (c_n)_{n \geq 1}$ given by

$$\begin{cases} b_n := \frac{1}{\sqrt{n^2}} + \cdots + \frac{1}{\sqrt{n^2}} \\ c_n := \frac{1}{\sqrt{N^2+n}} + \cdots + \frac{1}{\sqrt{N^2+n}} \end{cases}$$

Clearly, $\begin{cases} (b_n) \leq (a_n) \\ (c_n) \geq (a_n) \end{cases}$ for all $n \geq 1$.

Then one can easily find out the limit for both (b_n) and (c_n) , which can be calculated as

$$\lim_{n \rightarrow \infty} b_n = \lim_{n \rightarrow \infty} \sum_{k=1}^n \frac{1}{\sqrt{n^2}} = \lim_{n \rightarrow \infty} \sum_{k=1}^n \frac{1}{n} = \lim_{n \rightarrow \infty} \frac{n}{n} = \lim_{n \rightarrow \infty} 1 = 1$$

8.(continue)

$$\lim_{n \rightarrow \infty} c_n = \lim_{n \rightarrow \infty} \sum_{k=1}^n \frac{1}{\sqrt{n^2 + n}} = \lim_{n \rightarrow \infty} \frac{n}{\sqrt{n^2 + n}} = \lim_{n \rightarrow \infty} \frac{1}{\sqrt{1 + \frac{1}{n}}} = 1$$

By Squeeze Theorem, we know

$$\lim_{n \rightarrow \infty} b_n \leq \lim_{n \rightarrow \infty} a_n \leq \lim_{n \rightarrow \infty} c_n$$

, namely

$$1 \leq \lim_{n \rightarrow \infty} a_n \leq 1$$

We conclude that $\lim_{n \rightarrow \infty} a_n = 1$ ■

9. Prove that $\lim \sqrt[n]{n} = 1$.

9.

We consider the case for $n \geq 2$. Since $\sqrt[n]{n} > 1$ for all $n \geq 2$, we can choose a non-negative sequence, let say $(b_n)_{n \geq 2}$ such that

$$1 + b_n = \sqrt[n]{n}$$

From the fact that

$$(1 + b_n)^n = \sum_{k=0}^n \binom{n}{k} 1^k \cdot b_n^{n-k}$$

and another fact that $(1 + b_n)^n = n$, we get the following inequality

$$n = (1 + b_n)^n \leq \binom{n}{2} b_n^2 = \frac{n(n-1)}{2} b_n^2$$

9.(*continue*)

After some algebraic works, one can see

$$b_n \leq \sqrt{\frac{2}{n-1}}$$

But this means

$$0 \leq \sqrt[n]{n} - 1 \leq \sqrt{\frac{2}{n-1}}$$

By taking the limit, we have

$$0 \leq \lim_{n \rightarrow \infty} (\sqrt[n]{n} - 1) \leq \lim_{n \rightarrow \infty} \sqrt{\frac{2}{n-1}} = 0$$

9.(continue)

Finally, by Squeeze theorem, we get

$$\lim_{n \rightarrow \infty} (\sqrt[n]{n} - 1) = \lim_{n \rightarrow \infty} \sqrt[n]{n} - 1 = 0$$

We conclude

$$\lim_{n \rightarrow \infty} \sqrt[n]{n} = 1$$



End

Have Fun and Learn Well!